Proof that substitution gives sorts
Also better induction, decidable equality on types

proofs/core/Types.v
@@ -2,7 +2,93 @@ Require Export Coq.Strings.String.
 Require Export Coq.ZArith.BinInt.
 Require Export Coq.Arith.PeanoNat.
 Require Export Coq.Lists.List.
+Require Export Coq.Bool.Bool.
+Require Export Lia.
 Export ListNotations.
+
+Coercion proj_sumbool (A B: Prop) (H: {A} + {B}) : bool :=
+    if H then true else false.
+Coercion is_true : bool >-> Sortclass.
+
+(*TODO: move*)
+
+(*Union on lists with decidable equality*)
+Section Union.
+Context {A: Type}.
+Variable eq_dec: forall (x y : A), {x = y} + {x <> y}.
+
+(*Add all elements in l1 not in l2*)
+Definition union (l1 l2: list A) :=
+    fold_right (fun x acc => if in_dec eq_dec x acc then acc else x :: acc) l2 l1.
+
+Lemma union_nodup: forall (l1 l2: list A),
+  NoDup l2 ->
+  NoDup (union l1 l2).
+Proof.
+  intros l1 l2. induction l1; simpl; auto.
+  intros Hnodup.
+  destruct (in_dec eq_dec a (union l1 l2)); auto.
+  apply NoDup_cons; auto.
+Qed.
+
+Ltac solve_or :=
+  match goal with
+  | |- ?P \/ ?Q => first[left; solve_or | right; solve_or]
+  | |- ?P => solve[auto; try reflexivity]
+  end.
+
+Lemma union_elts: forall (l1 l2: list A) (x: A),
+  In x (union l1 l2) <-> In x l1 \/ In x l2.
+Proof.
+  intros l1 l2. induction l1; simpl; auto.
+  - intros x; split; intros; auto. destruct H as [[] |]; auto.
+  - intros x; split; intros Hin; destruct (in_dec eq_dec a (union l1 l2)).
+    + apply IHl1 in Hin. destruct Hin; solve_or.
+    + destruct Hin; subst; try solve_or. apply IHl1 in H; destruct H; solve_or.
+    + apply IHl1. destruct Hin as [Hin |?]; [destruct Hin; subst |]; try solve_or.
+      apply IHl1; auto.
+    + simpl. destruct Hin as [Hin|?]; [destruct Hin; subst|]; try solve_or.
+      all: right; apply IHl1; solve_or.
+Qed.
+
+Lemma union_remove: forall (l1 l2: list A) (x: A),
+  union (remove eq_dec x l1) (remove eq_dec x l2) =
+  remove eq_dec x (union l1 l2).
+Proof.
+  intros l1 l2. induction l1; simpl; auto.
+  intros x. destruct (eq_dec x a); subst.
+  - destruct (in_dec eq_dec a (union l1 l2)); simpl.
+    + apply IHl1.
+    + destruct (eq_dec a a); auto. contradiction.
+  - simpl. destruct (in_dec eq_dec a (union l1 l2)).
+    + destruct (in_dec eq_dec a (union (remove eq_dec x l1) (remove eq_dec x l2))); auto.
+      exfalso. apply n0. rewrite IHl1. apply in_in_remove; auto.
+    + simpl. destruct (eq_dec x a); subst; try contradiction.
+      destruct (in_dec eq_dec a (union (remove eq_dec x l1) (remove eq_dec x l2))); auto;
+      [| rewrite IHl1; auto].
+      exfalso. apply n0. rewrite IHl1 in i. apply in_remove in i. destruct i; auto.
+Qed.
+
+(*Iterated union*)
+Definition big_union {B: Type} (f: B -> list A) (l: list B) :=
+  fold_right (fun x acc => union (f x) acc) nil l.
+  
+Lemma big_union_nodup: forall {B: Type} (f: B -> list A) (l: list B),
+  NoDup (big_union f l).
+Proof.
+  intros. unfold big_union.
+  remember nil as base. assert (NoDup base) by (subst; constructor).
+  clear Heqbase. generalize dependent base.
+  induction l; simpl; auto.
+  intros base Hbase. apply union_nodup. apply IHl. auto.
+Qed.
+
+
+End Union.
+
+(*TODO: move*)
+(*Lemma NoDup_remove: 
+*)
 
 (*Type variable (ex: a)*)
 Definition typevar : Type := string. 
@@ -23,6 +109,7 @@ Proof.
 Defined.
 
 (*Value types*)
+Unset Elimination Schemes.
 Inductive vty : Type :=
   | vty_int : vty
   | vty_real : vty
@@ -31,11 +118,96 @@ Inductive vty : Type :=
   | vty_pred: vty -> vty*)
   (*| vty_tuple: vty -> vty -> vty*)
   | vty_var: typevar -> vty
-  | vty_cons: typesym -> list vty -> vty. (*TODO: do we need this? Can we make it non-list?*)
+  | vty_cons: typesym -> list vty -> vty.
+Set Elimination Schemes.
+
+(*Induction for this type*)
+Section TyInd.
+Variable P : vty -> Prop.
+Variable Hint: P vty_int.
+Variable Hreal: P vty_real.
+Variable Hvar: forall v, P (vty_var v).
+Variable Hcons: forall tsym vs,
+  Forall P vs -> P (vty_cons tsym vs).
+
+Fixpoint vty_ind (t: vty) : P t :=
+  match t with
+  | vty_int => Hint
+  | vty_real => Hreal
+  | vty_var t => Hvar t
+  | vty_cons tsym vs => Hcons tsym vs
+    ((fix vty_ind_list (l: list vty) : Forall P l :=
+      match l with
+      | nil => Forall_nil _
+      | x :: t => Forall_cons _ (vty_ind x) (vty_ind_list t)
+      end) vs)
+  end.
+
+End TyInd.
+
+(*Decidable equality on types*)
+
+Ltac simpl_sumbool :=
+    match goal with
+    | [H: is_true (proj_sumbool ?x ?y ?z) |- _ ] => destruct z; inversion H; clear H; subst; auto
+    | [H: (proj_sumbool ?x ?y ?z) = true |- _ ] => destruct z; inversion H; clear H; subst; auto
+    | |- is_true (proj_sumbool ?x ?y ?z) => destruct z; subst; auto
+    | |- (proj_sumbool ?x ?y ?z) = true => destruct z; subst; auto
+    end.
+
+Fixpoint vty_eqb (t1 t2: vty) : bool :=
+  match t1, t2 with
+  | vty_int, vty_int => true
+  | vty_real, vty_real => true
+  | vty_var t1, vty_var t2 => typevar_eq_dec t1 t2
+  | vty_cons ts1 vs1, vty_cons ts2 vs2 =>
+    typesym_eq_dec ts1 ts2 &&
+    ((fix vty_eqb_list (l1 l2: list vty) : bool :=
+      match l1, l2 with
+      | nil, nil => true
+      | x1 :: t1, x2 :: t2 => vty_eqb x1 x2 && vty_eqb_list t1 t2
+      | _, _ => false
+      end) vs1 vs2)
+  | _, _ => false
+  end.
+
+Lemma vty_eqb_eq: forall t1 t2,
+  vty_eqb t1 t2 -> t1 = t2.
+Proof.
+  intros t1. induction t1; simpl; auto; intros; destruct t2; auto; 
+  try match goal with
+  | H : is_true false |- _ => inversion H
+  end; try simpl_sumbool.
+  apply andb_prop in H0. destruct H0.
+  simpl_sumbool. f_equal. generalize dependent l. induction vs; simpl;
+  auto; intros; destruct l; auto; try solve[inversion H1].
+  inversion H; subst.
+  apply andb_prop in H1. destruct H1.
+  apply H3 in H0; subst. f_equal.
+  apply IHvs; auto.
+Qed.
+
+Lemma vty_eq_eqb: forall t1 t2,
+  t1 = t2 ->
+  vty_eqb t1 t2.
+Proof.
+  intros t1. induction t1; simpl; auto; intros; destruct t2; auto; try solve[inversion H];
+  try solve[inversion H0].
+  - inversion H; subst. simpl_sumbool.
+  - inversion H0; subst. apply andb_true_intro; split; [simpl_sumbool |].
+    clear H0. induction l; simpl; auto.
+    inversion H; subst. apply andb_true_intro; split; auto.
+    apply H2; auto.
+Qed. 
 
 Definition vty_eq_dec: forall (v1 v2: vty), {v1 = v2} + {v1 <> v2}.
-Admitted.
-(*TODO: need better induction*)
+Proof.
+  intros v1 v2. destruct (vty_eqb v1 v2) eqn : Heq.
+  - apply vty_eqb_eq in Heq. subst. left. auto.
+  - right. intro; subst. 
+    assert (vty_eqb v2 v2 = true) by (apply vty_eq_eqb; auto).
+    rewrite H in Heq; inversion Heq.
+Defined.
 
 (*Type substitution (assign meaning to a type variables)*)
 Fixpoint ty_subst_single (v: typevar) (t: vty) (expr: vty) : vty :=
@@ -56,14 +228,23 @@ Definition ty_subst_list (vs: list typevar) (ts: list vty) (exprs: list vty) : l
 
 (* Sorts *)
 
-(*Get the type variables in a type. There may be duplicates, but that is fine*)
+(*Get the type variables in a type, with no duplicates*)
 Fixpoint type_vars (t: vty) : list typevar :=
   match t with
   | vty_int => nil
   | vty_real => nil
   | vty_var v => [v]
-  | vty_cons sym ts => fold_right (fun x acc => type_vars x ++ acc) nil ts
+  | vty_cons sym ts => big_union typevar_eq_dec type_vars ts
   end.
+
+(*TODO: might be easier to do with ssreflect/undup*)
+Lemma type_vars_unique: forall t,
+  NoDup (type_vars t).
+Proof.
+  destruct t; simpl; try solve[constructor].
+  - constructor; auto. constructor.
+  - apply big_union_nodup.
+Qed.  
   
 Definition is_sort (t: vty) : bool :=
   match (type_vars t) with
@@ -71,26 +252,135 @@ Definition is_sort (t: vty) : bool :=
   | _ => false
   end.
 
-Definition sort : Type := {t: vty | is_true (is_sort t)}.
+Definition sort : Type := {t: vty | is_sort t}.
 (*TODO: see if we need an alternate definition*)
+Coercion sort_to_ty (s: sort) : vty := @proj1_sig _ _ s.
 
-Lemma int_is_sort: is_true (is_sort vty_int).
+Definition sorts_to_tys (l: list sort) : list vty :=
+  map sort_to_ty l.
+
+Lemma int_is_sort: is_sort vty_int.
 Proof.
   unfold is_sort; simpl. auto.
 Qed.
 
 Definition s_int : sort := exist _ vty_int int_is_sort.
 
-Lemma real_is_sort: is_true (is_sort vty_real).
+Lemma real_is_sort: is_sort vty_real.
 Proof.
   unfold is_sort; simpl. auto.
 Qed.
 
 Definition s_real : sort := exist _ vty_real real_is_sort.
 
+Lemma sort_type_vars: forall (s: sort),
+  type_vars s = nil.
+Proof.
+  intros s. destruct s; simpl. unfold is_sort in i.
+  destruct (type_vars x); auto. inversion i.
+Qed. 
+
 Definition sublist {A: Type} (l1 l2: list A) : Prop :=
     forall x, In x l1 -> In x l2.
 
 (*We want to know that when we substitute in sorts for type variables,
   the result is a sort *)
-(*TODO: this - after we have better induction principle for types*)
+
+Lemma ty_subst_single_sort: forall (v: typevar) (s: sort) (expr: vty),
+  type_vars (ty_subst_single v s expr) =
+  remove typevar_eq_dec v (type_vars expr).
+Proof.
+  intros v s expr. induction expr; simpl; auto.
+  - destruct (typevar_eq_dec v v0); simpl; auto.
+    apply sort_type_vars.
+  - induction vs; simpl; auto.
+    inversion H; subst. rewrite H2, IHvs; auto.
+    apply union_remove.
+Qed.
+
+(*Now, we lift this result to a list*)
+
+(*TODO: move*)
+(*Remove all elements of l1 from l2*)
+Definition remove_all {A: Type} (eq_dec: forall (x y : A), {x = y} + { x <> y })
+  (l1 l2: list A) :=
+  fold_right (remove eq_dec) l2 l1.
+
+Lemma ty_subst_remove_all: forall (vs: list typevar) (ss: list sort) (expr: vty),
+  length vs = length ss ->
+  type_vars (ty_subst vs (sorts_to_tys ss) expr) =
+  remove_all typevar_eq_dec vs (type_vars expr).
+Proof.
+  intros vs ss expr. revert ss. induction vs; simpl; intros.
+  symmetry in H. apply length_zero_iff_nil in H; subst; reflexivity.
+  destruct ss as [|s ss]; inversion H; subst.
+  simpl. unfold ty_subst in *; simpl.
+  rewrite ty_subst_single_sort. f_equal. apply IHvs. assumption.
+Qed.
+
+Lemma remove_filter: forall {A: Type} (eq_dec: forall (x y : A), {x = y} + { x <> y})
+  x l1,
+  remove eq_dec x l1 = filter (fun y => if eq_dec x y then false else true) l1.
+Proof.
+  intros. induction l1; simpl; intros; auto.
+  destruct (eq_dec x a); simpl; auto. rewrite IHl1; auto.
+Qed.
+
+Lemma remove_all_filter: forall {A: Type} (eq_dec: forall (x y : A), {x = y} + { x <> y })
+(l1 l2: list A),
+  remove_all eq_dec l1 l2 = filter (fun x => if in_dec eq_dec x l1 then false else true) l2.
+Proof.
+  intros. revert l2. induction l1; simpl; intros; auto.
+  - induction l2; simpl; intros; auto. rewrite IHl2 at 1; auto.
+  - rewrite IHl1, remove_filter. clear IHl1.
+    induction l2; simpl; intros; auto.
+    destruct (eq_dec a a0); subst; simpl.
+    + destruct (in_dec eq_dec a0 l1); subst; simpl; auto.
+      destruct (eq_dec a0 a0); subst; simpl; try contradiction.
+      apply IHl2.
+    + destruct (in_dec eq_dec a0 l1); subst; simpl; auto.
+      destruct (eq_dec a a0); subst; simpl; auto; try contradiction.
+      rewrite IHl2; reflexivity.
+Qed.
+
+Lemma sublist_nil: forall {A: Type} (l: list A),
+  sublist l nil ->
+  l = nil.
+Proof.
+  intros A l. destruct l; simpl; auto; unfold sublist.
+  intros H. specialize (H a). assert (In a nil) by (apply H; left; auto).
+  inversion H0.
+Qed.
+
+Lemma filter_nil: forall {A: Type} (f: A -> bool) (l: list A),
+  (forall x, In x l -> f x = false) ->
+  filter f l = nil.
+Proof.
+  intros A f l. induction l; simpl; intros; auto.
+  rewrite H; [|left; auto]. apply IHl.
+  intros x Hinx. apply H. right; auto.
+Qed. 
+
+Lemma remove_all_sublist: forall {A: Type} (eq_dec: forall (x y : A), {x = y} + { x <> y })
+(l1 l2: list A),
+  sublist l2 l1 ->
+  remove_all eq_dec l1 l2 = nil.
+Proof.
+  intros. rewrite remove_all_filter.
+  apply filter_nil. unfold sublist in H.
+  intros x Hinx. apply H in Hinx.
+  destruct (in_dec eq_dec x l1); try contradiction. reflexivity.
+Qed.
+
+(*Finally, we get the result we want*)
+
+Lemma ty_subst_sort: forall (vs: list typevar) (ts: list sort) (expr: vty),
+  length vs = length ts ->
+  (sublist (type_vars expr) vs) ->
+  is_sort (ty_subst vs (sorts_to_tys ts) expr).
+Proof.
+  intros vs ts expr Hlens Hsub. unfold is_sort.
+  assert (Hvars: type_vars (ty_subst vs (sorts_to_tys ts) expr) = nil); [|rewrite Hvars; auto].
+  rewrite ty_subst_remove_all; auto.
+  apply remove_all_sublist; auto.
+Qed.
